Remove outdated s/\ notation

theories/Mon/README.v
@@ -186,10 +186,10 @@ Section NonDeterminism.
     Fixpoint and (xs : list SProp) : SProp :=
       match xs with
       | nil => True
-      | P :: Ps => P s/\ and Ps
+      | P :: Ps => P /\ and Ps
       end.
 
-    Lemma and_app : forall l1 l2, and (l1 ++ l2) = (and l1 s/\ and l2).
+    Lemma and_app : forall l1 l2, and (l1 ++ l2) = (and l1 /\ and l2).
     Proof.
       intros l1 l2. apply SPropAxioms.sprop_ext.
       induction l1; simpl; constructor; intuition.
@@ -341,7 +341,7 @@ Section DijkstraState.
      post conditions. *)
   Program Definition PrePostWP (P : S -> SProp) (Q : S -> S -> SProp)
     : StateSpec unit :=
-    fun s0 => ⦑fun (Z : unit × S -> SProp) => P s0 s/\ forall s1, Q s0 s1 -> Z ⟨tt, s1⟩⦒.
+    fun s0 => ⦑fun (Z : unit × S -> SProp) => P s0 /\ forall s1, Q s0 s1 -> Z ⟨tt, s1⟩⦒.
   Next Obligation. intuition eauto ; move: (q s1 H0) ; apply H. Qed.
 
   Definition PrePost P (Q : S -> S -> SProp) :=
@@ -412,7 +412,7 @@ Section DemonicNonDeterminism.
     ifTE b (dret tt) failD.
 
   Program Definition test_demonic
-    : Demonic nat (PostDemonic (fun x => 1 < x s/\ x < 6))
+    : Demonic nat (PostDemonic (fun x => 1 < x /\ x < 6))
     := wkn (chooseD (2 :: 3 :: 5 :: nil)) _.
   Next Obligation.
     simpl in *.
@@ -454,7 +454,7 @@ Section IO.
   Definition write' (o : Oup) : IO unit _ := lift _ (write _ o).
 
   Program Definition mustHaveOccurredSpec (o : Oup) : IOSpec unit :=
-    fun history => ⦑fun post => Squash (In (existT _ (Write o) tt) history) s/\ post ⟨tt, history⟩ ⦒.
+    fun history => ⦑fun post => Squash (In (existT _ (Write o) tt) history) /\ post ⟨tt, history⟩ ⦒.
   Next Obligation.
     move: H0 ; simpl ; intuition.
   Qed.
@@ -752,7 +752,7 @@ Section Exceptions.
 
     Import SPropNotations.
     Program Definition PrePostExcSpec {A} (P : SProp) (Q : A -> SProp) : ExcSpec A :=
-      ⦑fun (Z : A -> SProp) => P s/\ forall a, Q a -> Z a⦒.
+      ⦑fun (Z : A -> SProp) => P /\ forall a, Q a -> Z a⦒.
     Next Obligation. cbv ; intuition. Qed.
 
     Definition PrePostExc {A} P (Q : A -> SProp) :=
@@ -780,8 +780,8 @@ Section Exceptions.
     ExcSpec Q_exn' B
     :=
       fun P Q Q_exn wp_ret wp_exn =>
-        ⦑fun post => P s/\ (forall a, Q a -> proj1_sig (wp_ret a) post)
-                  s/\ (Q_exn -> proj1_sig wp_exn post)⦒.
+        ⦑fun post => P /\ (forall a, Q a -> proj1_sig (wp_ret a) post)
+                  /\ (Q_exn -> proj1_sig wp_exn post)⦒.
   Next Obligation.
     destruct H0 as [[]] ; intuition.
   Qed.
