theories/Crypt/rules/Theta_forall.v
@@ -282,7 +282,7 @@ Proof.
   rewrite /SDistr_carrier. move => [d1 d2].
   exists (fun π : A1 * A2 -> SProp => (s∀ d, Prop2SProp (coupling d d1 d2) ->
                                     (s∃ (a1 : A1) (a2 : A2),
-                                          (π (a1, a2)) s/\ (d (a1, a2) > 0 ≡ true)))).
+                                          (π (a1, a2)) /\ (d (a1, a2) > 0 ≡ true)))).
   move => π1 π2 leq12 H d coup_d.
   move: (H d coup_d).
   move => [a1 [a2 [Hπ2 Hd]]].
@@ -322,7 +322,7 @@ Axiom indefinite_Sdescription : forall {A : Type} (P : A -> SProp),
 (*                          s∃ d : SDistr_carrier (Couplings.F_choice_prod_obj *)
 (*                                                   ⟨ Choice.Pack chB1, Choice.Pack chB2 ⟩), *)
 (*                              Prop2SProp (coupling d (f1 a1) (f2 a2)) *)
-(*                                         s/\ (forall (a3 : B1) (a4 : B2), 0 < d (a3, a4) -> π (a3, a4))) : *)
+(*                                         /\ (forall (a3 : B1) (a4 : B2), 0 < d (a3, a4) -> π (a3, a4))) : *)
 (*        TypeCat ⦅ choice_incl (F_choice_prod ⟨ Choice.Pack chA1, Choice.Pack chA2 ⟩); *)
 (*                  SDistr (F_choice_prod ⟨ Choice.Pack chB1, Choice.Pack chB2 ⟩) ⦆. *)
 (* Proof. *)
@@ -352,7 +352,7 @@ Axiom indefinite_Sdescription : forall {A : Type} (P : A -> SProp),
 (*                   s∃ d : SDistr_carrier (Couplings.F_choice_prod_obj *)
 (*                                            ⟨ Choice.Pack chB1, Choice.Pack chB2 ⟩), *)
 (*                       Prop2SProp (coupling d (f1 a1) (f2 a2)) *)
-(*                                  s/\ (forall (a3 : B1) (a4 : B2), 0 < d (a3, a4) -> π (a3, a4))) : *)
+(*                                  /\ (forall (a3 : B1) (a4 : B2), 0 < d (a3, a4) -> π (a3, a4))) : *)
 (*   (forall (x1 : A1) (x2 : A2), coupling ((kd dA integral) (x1,x2)) (f1 x1) (f2 x2)). *)
 (* Proof. *)
 (*   move => a1 a2. *)
